wip

core/RefinementUpdate.v
@@ -7,57 +7,107 @@ Require Import FunctionalExtensionality.
 Require Import ExtensionalUpdate.
 Import ListNotations.
 
+Set Bullet Behavior "Strict Subproofs".
 
-Section RefinementUpdate.
+
+Section SimulationUpdate.
   Context `{params : SimpleUpdateParams}.
 
-  Variable refinements :
+  Variable first_update : handlerUpdate P.
+  Variable first_update_first : Nth updates 0 first_update.
+
+  Variable simulations :
     list (data -> data -> Prop).
 
-  Variable refinements_valid :
+  Variable simulations_valid :
     forall n update,
       Nth updates (S n) update ->
-      exists refinement,
-        Nth refinements n refinement.
+      exists simulation,
+        Nth simulations n simulation.
 
-  Variable update_establishes_refinement :
-    forall n update up failed net h out d ms refinement,
+  Variable update_establishes_simulation :
+    forall n update up failed net h out d ms simulation,
       su_reachable_state (up, failed, net) ->
       up h = n ->
       Nth updates (S n) update ->
       huUpdate update h (nwState net h) = (out, d, ms) ->
-      Nth refinements n refinement ->      
+      Nth simulations n simulation ->      
       out = nil /\
       ms = nil /\
-      refinement (nwState net h) d.
+      simulation (nwState net h) d.
 
-  Definition equiv_mod_host h (st st' : (name -> nat) * list name * network) :=
-    (forall h',
-        h <> h' ->
-        (fst (fst st)) h' = (fst (fst st')) h') /\
-    snd (fst st) = snd (fst st') /\
-    (forall h',
-        h <> h' ->
-        nwState (snd st) h' = nwState (snd st') h') /\
-    nwPackets (snd st) = nwPackets (snd st').
-
-  Variable input_handlers_preserve_refinements :
-    forall n update1 update2 st st' h inp out d ms out' d' ms' refinement,
+  Variable input_handlers_preserve_simulations :
+    forall n update1 update2 st st' h inp out d ms out' d' ms' simulation,
       su_reachable_state st ->
       su_reachable_state st' ->
       (fst (fst st)) h = n ->
       (fst (fst st')) h = S n ->
       Nth updates n update1 ->
       Nth updates (S n) update2 ->
-      Nth refinements n refinement ->
-      refinement (nwState (snd st) h) (nwState (snd st') h) ->
+      Nth simulations n simulation ->
+      simulation (nwState (snd st) h) (nwState (snd st') h) ->
       huInput update1 h inp (nwState (snd st) h) = (out, d, ms) ->
       huInput update2 h inp (nwState (snd st') h) = (out', d', ms') ->
-      refinement d d' /\ out = out' /\ ms = ms'.
+      simulation d d' /\ out = out' /\ ms = ms'.
 
-  Variable first_update : handlerUpdate P.
-  Variable first_update_first : Nth updates 0 first_update.
+  Inductive path : nat -> data -> data -> Prop :=
+  | pathO : forall st, path 0 st st
+  | pathS :
+      forall n simulation st st' st'',
+        path n st st' ->
+        Nth simulations n simulation ->
+        simulation st' st'' ->
+        path (S n) st st''.
+
+  Lemma Nth_S_Nth :
+    forall A (l : list A) n x,
+      Nth l (S n) x ->
+      exists y,
+        Nth l n y.
+  Proof.
+    induction l.
+    - intros.
+      invcs H.
+    - intros.
+      invcs H.
+      destruct n.
+      + eexists; econstructor.
+      + find_apply_hyp_hyp.
+        break_exists_exists. constructor. auto.
+  Qed.
+      
+  Lemma input_handlers_preserve_paths :
+    forall n update2 st st' h inp out d ms out' d' ms',
+      path n (nwState (snd st) h) (nwState (snd st') h) ->
+      su_reachable_state st ->
+      su_reachable_state st' ->
+      Nth updates n update2 ->
+      huInput first_update h inp (nwState (snd st) h) = (out, d, ms) ->
+      huInput update2 h inp (nwState (snd st') h) = (out', d', ms') ->
+      path n d d' /\ out = out' /\ ms = ms'.
+  Proof.
+    induction n (* path *); intros; simpl in *;
+      match goal with
+      | H : path _ _ _ |- _ =>
+        invcs H
+      end.
+    - repeat find_apply_lem_hyp Nth_nth_error.
+      repeat find_rewrite.
+      find_injection.
+      repeat find_rewrite.
+      tuple_inversion.
+      intuition.
+      constructor.
+    - find_copy_apply_lem_hyp Nth_S_Nth.
+      break_exists_name update1.
+      
+      
   
+  Definition equiv_states (st st' : (name -> nat) * list name * network) :=
+    (forall h,
+        path ((fst (fst st')) h) (nwState (snd st) h) (nwState (snd st') h)) /\
+    snd (fst st) = snd (fst st') /\
+    nwPackets (snd st) = nwPackets (snd st').
   
   Definition multi_updates := updates.
 
@@ -69,5 +119,50 @@ Section RefinementUpdate.
   Notation step_one_star := (@step_u_star _ _ _ one_update_params).
   Notation step_multi_star := (@step_u_star _ _ _ params).
 
-  Fixpoint refinement_path n ->
-  
+  Definition is_reachable_equiv_state (st : (name -> nat) * list name * network) :=
+    exists st' tr,
+      step_one_star step_u_init st' tr /\
+      equiv_states st' st.
+
+  Definition step_multi_step_one :
+    forall sto sto' stm trm tro tro',
+      step_multi_star step_u_init stm trm ->
+      step_one_star step_u_init sto tro ->
+      step_one sto sto' tro' ->
+      equiv_states sto stm ->
+      exists stm' trm',
+        equiv_states sto' stm' /\
+        step_multi stm stm' trm'.
+  Proof.
+    intros.
+    invcs H1.
+    - match goal with
+      | H : Nth [_] _ _ |- _ => invcs H; [|solve_by_inversion]
+      end.
+      
+      
+
+
+  Theorem is_reachable_equiv_state_inductive :
+    inductive_invariant step_multi step_u_init is_reachable_equiv_state.
+  Proof.
+    unfold inductive_invariant.
+    intuition;
+      [(exists step_u_init, []); cbn; intuition;
+       constructor; intuition; constructor|].
+    unfold inductive. intros. invcs H0.
+    - admit.
+    - unfold is_reachable_equiv_state in *.
+      break_exists_name st'; break_exists. intuition.
+      destruct st', p.
+      match goal with
+      | H: context [equiv_states] |- _ =>
+        unfold equiv_states in H
+      end. simpl in *. intuition. subst.
+      exists (n0, failed, {|
+           nwPackets := map
+                          (fun m : name * msg =>
+                             {| pSrc := h; pDst := fst m; pBody := snd m |}) l ++
+                          nwPackets n;
+           nwState := fun nm : name => if name_eq_dec nm h then d else nwState n nm |}).
+      exists x.
